Added some lemmas

logic.lean
@@ -4,7 +4,10 @@ import .types
 
 universes u v
 
+noncomputable theory
+
 notation `⊥` :=  ∀p: Prop, p
+notation `⊤` := ¬⊥
 
 def not (p: Prop) := p → ⊥
 
@@ -25,11 +28,12 @@ instance Prop_vee_Prop: has_vee Prop Prop Prop :=
 
 structure iff (p q: Prop) : Prop :=
   intro :: (mp: p → q) (mpr: q → p)
-instance Prop_leftrightarrow_Pro: has_leftrightarrow Prop Prop Prop := ⟨iff⟩
+instance Prop_leftrightarrow_Prop: has_leftrightarrow Prop Prop Prop := ⟨iff⟩
 
 def equ {α: Sort u} (a b: α) : Prop := ∀ϕ: α → Prop, ϕ a ↔ ϕ b
 instance homo_eq(α: Sort u): has_eq α α Prop := ⟨equ⟩
 def neq {α: Sort u} (a b: α) := ¬(a = b)
+instance homo_neq(α: Sort u): has_ne α α Prop := ⟨neq⟩
 
 inductive Exists {α: Sort u} (ϕ: α → Prop) : Prop
   | intro (a: α) (h: ϕ a) : Exists
@@ -38,3 +42,88 @@ notation `∃` binders `, ` r:(scoped P, Exists P) := r
 def exists_unique {α: Sort u} (ϕ: α → Prop) :=
   ∃ x, ϕ x ∧ ∀ y, ϕ y → y = x
 notation `∃!` binders `, ` r:(scoped P, exists_unique P) := r
+
+lemma dn_intro {p: Prop} : p → ¬¬p :=
+  λhp: p,
+    λhnp: ¬p,
+      hnp hp
+lemma and.elim_left {p q: Prop} : p∧q → p :=
+  λh: p ∧ q,
+    h.left
+lemma and.elim_right {p q: Prop} : p∧q → q :=
+  λh: p ∧ q,
+    h.right
+lemma or.intro_left {p: Prop} (q: Prop) : p → p∨q :=
+  λhp: p,
+    or.inl hp
+lemma or.intro_right (p: Prop) {q: Prop} : q → p∨q :=
+  λhq: q,
+    or.inr hq
+lemma iff.elim_left {p q: Prop} : (p↔q) → p→q :=
+  λh: p↔q,
+    h.mp
+lemma iff.elim_right {p q: Prop} : (p↔q) → q→p :=
+  λh: p↔q,
+    h.mpr
+lemma equ.refl {α: Sort u} (a: α) : a = a :=
+  λϕ: α → Prop,
+    iff.intro
+      (λh: ϕ a, h)
+      (λh: ϕ a, h)
+lemma equ.symm {α: Sort u} {a b: α}: a = b → b = a :=
+  λh: a = b,
+    λϕ: α → Prop,
+      iff.intro
+        (h ϕ).mpr
+        (h ϕ).mp
+lemma equ.trans {α: Sort u} {a b c: α}: a = b → b = c → a = c :=
+  λh₁: a = b,
+    λh₂: b = c,
+      λϕ: α → Prop,
+        iff.intro
+          (λhpa: ϕ a, (h₂ ϕ).mp ((h₁ ϕ).mp hpa)) --ϕ a → ϕ c
+          (λhpc: ϕ c, (h₁ ϕ).mpr ((h₂ ϕ).mpr hpc))--ϕ c → ϕ a
+lemma equ.subst {α: Sort u} (P: α → Prop) {a b: α}: a = b → (P a ↔ P b) := 
+  λh: a = b,
+    h P
+infixr ` ▸ `:75 := equ.subst
+lemma equ.comm {α: Sort u} {a b: α}: a=b ↔ b=a :=
+  iff.intro (λh: a=b, equ.symm h) (λh: b=a, equ.symm h)
+--
+def trivial: ⊤ := 
+  λf: ⊥, f
+def implies (p q: Prop) := p → q
+lemma implies.trans {p q r: Prop} : (p→q) → (q→r) → (p→r) := 
+  λh₁: p→q,
+    λh₂: q→r,
+      λhp: p,
+        h₂ (h₁ hp)
+def absurd {p: Prop} (h₁: p) (h₂: ¬p) (q: Prop) : q :=
+  h₂ h₁ q
+lemma mt {p q: Prop} : (p → q) → (¬q → ¬p) :=
+  λh: p → q,
+    λhnq: ¬q,
+      λhp: p,
+        hnq (h hp)
+lemma not_false: ¬⊥ := trivial
+lemma equ.mp {α β: Sort u} : (α = β) → (α → β) := sorry --Unsure
+lemma equ.mpr {α β: Sort u} : (α = β) → (β → α) := sorry --Unsure
+lemma equ.substr {α: Sort u} {P: α → Prop} {a b: α} : a = b → P a → P b := sorry
+lemma congr {α: Sort u} {β: Sort v} {f g: α → β} {a b: α}: f = g → a = b → f a = g b :=
+  λh₁: f = g,
+    λh₂: a = b,
+      λϕ: β → Prop,
+        iff.intro
+          (λhpfa: ϕ (f a), (h₂ (λa', ϕ (g a'))).mp ((h₁ (λf', ϕ (f' a))).mp hpfa)) --Leibnizian
+          (λhpgb: ϕ (g b), (h₂ (λb', ϕ (f b'))).mpr ((h₁ (λg', ϕ (g' b))).mpr hpgb)) --Chicanery
+
+lemma congr_fun {α: Sort u} {β: α → Sort v} {f g: Πx, β x} (h: f = g) (a: α) :
+  f a = g a := sorry
+lemma congr_arg {α: Sort u} {β: Sort v} {a b: α} (f: α → β) : a = b → f a = f b :=
+  congr (equ.refl f)
+lemma trans_rel_left {α: Sort u} {a b c: α} (r: α → α → Prop) :
+  r a b → b = c → r a c := sorry
+lemma trans_rel_right {α: Sort u} {a b c: α} (r: α → α → Prop) :
+  a = b → r b c → r a c := sorry
+lemma of_eq_true {p: Prop} (h: p = ⊤) : p := sorry
+lemma not_of_eq_false {p: Prop} (h: p = ⊥) : ¬p := sorry
